Adapted design refinement calculus with the things added to the relation version

theories/utp_refcalc.thy
@@ -3,7 +3,57 @@ section {* Refinement calculus *}
 theory utp_refcalc
   imports utp_designs
 begin
+  
+definition spec :: "('a \<Longrightarrow> '\<alpha>) \<Rightarrow> '\<alpha> upred \<Rightarrow> ('\<alpha> \<Rightarrow> '\<alpha> upred) \<Rightarrow> '\<alpha> hrel_des" where
+[upred_defs]: "spec x p q = (\<Squnion> v \<bullet> (\<lceil>p \<and> &\<^bold>v =\<^sub>u \<guillemotleft>v\<guillemotright>\<rceil>\<^sub>< \<turnstile>\<^sub>r x:[\<lceil>q(v)\<rceil>\<^sub>>]))"
 
+syntax
+  "_init_var"  :: "logic"
+  "_spec"      :: "salpha \<Rightarrow> logic \<Rightarrow> logic \<Rightarrow> logic" ("_:[_,/ _]" [99,0,0] 100)
+  "_log_const" :: "pttrn \<Rightarrow> logic \<Rightarrow> logic" ("con _ \<bullet> _" [0, 10] 10)
+  
+translations
+  "_spec x p q" => "CONST spec x p (\<lambda> _init_var. q)"
+  "_spec (_salphaset (_salphamk x)) p q" <= "CONST spec x p (\<lambda> iv. q)"
+  "_log_const x P" => "\<Squnion> x \<bullet> P"
+
+parse_translation {*
+let
+  fun init_var_tr [] = Syntax.free "iv"
+    | init_var_tr _  = raise Match;
+in
+[(@{syntax_const "_init_var"}, K init_var_tr)]
+end
+*}
+  
+abbreviation abort :: "'\<alpha> hrel_des" where
+"abort \<equiv> true"
+
+abbreviation magic :: "'\<alpha> hrel_des" where
+"magic \<equiv> \<top>\<^sub>D"
+
+abbreviation skip :: "'\<alpha> hrel_des" where
+"skip \<equiv> \<emptyset>:[true,true]"
+  
+abbreviation "chose x \<equiv> {&x}:[true,true]"
+
+  
+lemma spec_simple_def: 
+  "x:[pre,post] = (\<lceil>pre\<rceil>\<^sub>< \<turnstile>\<^sub>r x:[\<lceil>post\<rceil>\<^sub>>])"
+  by (rel_auto)
+  
+lemma spec_abort:
+  "x:[false,post] = true"
+  by (rel_auto)
+ 
+lemma spec_skip:
+  "\<emptyset>:[true,true] = skip"
+  by simp
+    
+lemma skip_des_skip: "skip = II\<^sub>D"
+  by (rel_auto)
+
+  
 abbreviation spec_stat :: "('\<beta> \<Longrightarrow> '\<alpha>) \<Rightarrow> '\<alpha> upred \<Rightarrow> '\<alpha> upred \<Rightarrow> '\<alpha> hrel_des" where
 "spec_stat w pre post \<equiv> (pre \<turnstile>\<^sub>n w:[\<lceil>post\<rceil>\<^sub>>])"
 
